Url.lean
@@ -19,3 +19,6 @@ import Url.Ipv4Roundtrip
 import Url.HostRoundtrip
 import Url.Ipv6Roundtrip
 import Url.SearchParams
+import Url.Spec.Failure
+import Url.Spec.Relative
+import Url.Spec.Priority
